src/ExprUnify.v
@@ -9,6 +9,39 @@ Set Strict Implicit.
 
 Module SUBST := NatMap.IntMap.
 
+Section fold_left2_opt.
+  Variable T U V : Type.
+  Variable F : T -> V -> U -> option U.
+
+  Fixpoint fold_left_2_opt (ls : list T) (ls' : list V) (acc : U) : option U :=
+    match ls, ls' with 
+      | nil , nil => Some acc
+      | x :: xs , y :: ys => 
+        match F x y acc with
+          | None => None
+          | Some acc => fold_left_2_opt xs ys acc
+        end
+      | _ , _ => None
+    end.
+End fold_left2_opt.
+
+Section fold_left3_opt.
+  Variable T U V A : Type.
+  Variable F : T -> U -> V -> A -> option A.
+
+  Fixpoint fold_left_3_opt (ls : list T) (ls' : list U) (ls'' : list V) 
+    (acc : A) : option A :=
+    match ls, ls', ls'' with 
+      | nil , nil , nil => Some acc
+      | x :: xs , y :: ys , z :: zs => 
+        match F x y z acc with
+          | None => None
+          | Some acc => fold_left_3_opt xs ys zs acc
+        end
+      | _ , _ , _ => None
+    end.
+End fold_left3_opt.
+
 Section Unify.
   Variable types : list type.
 
@@ -70,21 +103,6 @@ Section Unify.
    ** If uL is not nil, then this procedure is not even structurally complete
    **)
 
-  Section fold_left2_opt.
-    Variable T U V : Type.
-    Variable F : T -> V -> U -> option U.
-
-    Fixpoint fold_left_2_opt (ls : list T) (ls' : list V) (acc : U) : option U :=
-      match ls, ls' with 
-        | nil , nil => Some acc
-        | x :: xs , y :: ys => 
-          match F x y acc with
-            | None => None
-            | Some acc => fold_left_2_opt xs ys acc
-          end
-        | _ , _ => None
-      end.
-  End fold_left2_opt.
 
 
   Fixpoint exprUnify (l r : expr types) (ls rs : Subst) : option (Subst * Subst).
